Cross-chain collision and preimage, and start hash trees

Examples/XMSS/TweakableHashFunctions.lean
@@ -47,12 +47,12 @@ namespace TweakableHash
 def chain {PP TW X Y : Type}
     (thf : TweakableHash PP TW X Y)
     (outToIn : Y → X)
-    (twat : Nat → TW)
+    (twAt : Nat → TW)
     (pp : PP)
     (start steps : Nat)
     (x : Y) : Y :=
   idxIter
-    (fun pos y => thf pp (twat pos) (outToIn y))
+    (fun pos y => thf pp (twAt pos) (outToIn y))
     start
     steps
     x
@@ -61,38 +61,39 @@ def chain {PP TW X Y : Type}
 theorem chain_zero {PP TW X Y: Type}
     (thf : TweakableHash PP TW X Y)
     (outToIn : Y → X)
-    (twat : Nat → TW)
+    (twAt : Nat → TW)
     (pp : PP)
     (start : Nat)
     (x : Y) :
-    chain thf outToIn twat pp start 0 x = x :=
+    chain thf outToIn twAt pp start 0 x = x :=
   by rfl
 
 @[simp]
 theorem chain_succ {PP TW X Y: Type}
     (thf : TweakableHash PP TW X Y)
     (outToIn : Y → X)
-    (twat : Nat → TW)
+    (twAt : Nat → TW)
     (pp : PP)
     (start i : Nat)
     (x : Y) :
-    chain thf outToIn twat pp start (i + 1) x
+    chain thf outToIn twAt pp start (i + 1) x
     =
-    thf pp (twat (start + i)) (outToIn (chain thf outToIn twat pp start i x)) :=
+    thf pp (twAt (start + i)) (outToIn (chain thf outToIn twAt pp start i x)) :=
   by rfl
 
 theorem chain_comp {PP TW X Y: Type}
     (thf : TweakableHash PP TW X Y)
     (outToIn : Y → X)
-    (twat : Nat → TW)
+    (twAt : Nat → TW)
     (pp : PP)
     (start i j : Nat)
     (x : Y) :
-    chain thf outToIn twat pp start (i + j) x
+    chain thf outToIn twAt pp start (i + j) x
     =
-    chain thf outToIn twat pp (start + i) j (chain thf outToIn twat pp start i x) :=
+    chain thf outToIn twAt pp (start + i) j (chain thf outToIn twAt pp start i x) :=
   by
     simp [chain, idxIter_comp]
+
 
 def isColl {PP TW X Y: Type}
     (thf : TweakableHash PP TW X Y)
@@ -101,18 +102,19 @@ def isColl {PP TW X Y: Type}
     (x x' : X) : Prop :=
   x ≠ x' ∧ thf pp tw x = thf pp tw x'
 
-theorem chain_coll {PP TW X Y: Type}
+theorem chain_cross_coll {PP TW X Y: Type}
     (thf : TweakableHash PP TW X Y)
     (outToIn : Y → X)
-    (twat : Nat → TW)
+    (twAt : Nat → TW)
     (pp : PP)
     (start steps : Nat)
     (x x' : Y)
-    (outToIn_inj : Function.Injective outToIn)
-    (xxp_neq : x ≠ x'):
-    chain thf outToIn twat pp start steps x = chain thf outToIn twat pp start steps x' →
-    ∃i : Nat, i < steps ∧ isColl thf pp (twat (start + i)) (outToIn (chain thf outToIn twat pp start i x)) (outToIn (chain thf outToIn twat pp start i x')) :=
+    (outToIn_inj : Function.Injective outToIn) :
+    x ≠ x' →
+    chain thf outToIn twAt pp start steps x = chain thf outToIn twAt pp start steps x' →
+    ∃i : Nat, i < steps ∧ isColl thf pp (twAt (start + i)) (outToIn (chain thf outToIn twAt pp start i x)) (outToIn (chain thf outToIn twAt pp start i x')) :=
   by
+    intro xxp_neq
     induction steps with
     | zero =>
         simp only [chain_zero]
@@ -121,7 +123,7 @@ theorem chain_coll {PP TW X Y: Type}
     | succ steps ih =>
         intro heqnext
         by_cases hprev :
-          chain thf outToIn twat pp start steps x = chain thf outToIn twat pp start steps x'
+          chain thf outToIn twAt pp start steps x = chain thf outToIn twAt pp start steps x'
         · obtain ⟨i, hi, hcoll⟩ := ih hprev
           refine ⟨i, ?_, hcoll⟩
           exact Nat.lt_trans hi (Nat.lt_succ_self steps)
@@ -131,4 +133,32 @@ theorem chain_coll {PP TW X Y: Type}
             apply hprev
             exact outToIn_inj heqout
           · simpa only [chain_succ] using heqnext
+
+
+def isPre {PP TW X Y: Type}
+    (thf : TweakableHash PP TW X Y)
+    (pp : PP)
+    (tw : TW)
+    (x : X)
+    (y : Y) : Prop :=
+  thf pp tw x = y
+
+theorem chain_cross_pre {PP TW X Y: Type}
+    (thf : TweakableHash PP TW X Y)
+    (outToIn : Y → X)
+    (twAt : Nat → TW)
+    (pp : PP)
+    (start steps : Nat)
+    (x x' : Y) :
+    0 < steps →
+    chain thf outToIn twAt pp start steps x = chain thf outToIn twAt pp start steps x' →
+    isPre thf pp (twAt (start + steps - 1)) (outToIn (chain thf outToIn twAt pp start (steps - 1) x)) (chain thf outToIn twAt pp start steps x') :=
+  by
+    induction steps with
+    | zero =>
+        intro lt0_0
+        contradiction
+    | succ steps ih =>
+        intro lt0_steps1
+        simp [isPre, chain_succ]
 end TweakableHash
