Examples/XMSS/HashTrees.lean
@@ -1,0 +1,45 @@
+universe u
+
+inductive HashTree (H : Type u) where
+  | leaf (value : H)
+  | node (value : H) (left right : HashTree H)
+
+namespace HashTree
+
+variable {H : Type u}
+
+def value : HashTree H → H
+  | .leaf value => value
+  | .node value _ _ => value
+
+def height : HashTree H → Nat
+  | .leaf _ => 0
+  | .node _ l r => 1 + max (height l) (height r)
+
+def numLeaves : HashTree H → Nat
+  | .leaf _ => 1
+  | .node _ l r => l.numLeaves + r.numLeaves
+
+
+
+def IsPerfect : HashTree H → Prop
+  | .leaf _ => True
+  | .node _ l r => l.height = r.height ∧ l.IsPerfect ∧ r.IsPerfect
+
+def IsBalanced : HashTree H → Prop
+  | .leaf _ => True
+  | .node _ l r => (l.height - r.height) + (r.height - l.height) ≤ 1
+
+def IsPerfectlyBalanced : HashTree H → Prop
+  | .leaf _ => True
+  | .node _ l r => l.height = r.height
+
+/- def fromLeaves
+ -     (leaves : List H)
+ -     (f : Nat → Nat → H → H → H)
+ -     (idx : Nat × Nat) : HashTree H :=
+ -   f idx₁ idx₂
+ -     (fromLeaves (firstHalf leaves) f (idx₁ + 1, 2 * idx₂))
+ -     (fromLeaves (secondHalf leaves) f (idx₁ + 1, 2 * idx₁ + 1)) -/
+
+end HashTree
